Start using Asimpl in places

theories/FOL/Undecidability/Reductions/PCPb_to_binZF.v
@@ -1,6 +1,7 @@
 (** ** Translation from ZF over Skolem signature *)
 
 Require Import Undecidability.FOL.Syntax.Facts.
+Require Import Undecidability.FOL.Syntax.Asimpl.
 Require Import Undecidability.FOL.Semantics.Tarski.FullFacts.
 Require Import Undecidability.FOL.Deduction.FullNDFacts.
 From Undecidability.FOL.Sets Require Import binZF ZF.
@@ -50,8 +51,20 @@ Fixpoint embed {ff'} (phi : form sig_empty sig_binary _ ff') : form ff' :=
 
 (* ** Translation function *)
 
-Definition sshift {Σ_funcs : funcs_signature} k : nat -> term :=
+Definition sshift' {Σ_funcs : funcs_signature} k : nat -> term :=
   fun n => match n with 0 => $0 | S n => $(1 + k + n) end.
+Definition sshift {Σ_funcs : funcs_signature} k : nat -> term :=
+  $0 .: iter (fun k => S >> k) k (S >> var).
+
+Lemma sshift_spec {Σ_funcs : funcs_signature} k n : @sshift' Σ_funcs k n = sshift k n.
+Proof.
+  induction k as [|k IH] in n|-*.
+  - easy.
+  - destruct n as [|n].
+    + easy.
+    + cbn. specialize (IH (S (S n))). cbn in IH.
+      rewrite <- plus_n_Sm in IH. rewrite IH. easy.
+Qed.
 
 Fixpoint rm_const_tm (t : term) : form' :=
   match t with
@@ -179,14 +192,14 @@ Section Model.
     induction phi in sigma |- *; cbn; trivial.
     - f_equal. erewrite !Vector.map_map, Vector.map_ext. reflexivity. apply embed_subst_t.
     - firstorder congruence.
-    - rewrite IHphi. f_equal. apply subst_ext. intros []; cbn; trivial.
+    - rewrite IHphi. asimpl. f_equal. apply subst_ext. intros []; cbn; trivial.
       unfold funcomp. cbn. unfold funcomp. now destruct (sigma n) as [x|[]].
   Qed.
 
   Lemma embed_sshift n (phi : form') :
     embed phi[sshift n] = (embed phi)[sshift n].
   Proof.
-    rewrite embed_subst. apply subst_ext. now intros [].
+    rewrite embed_subst. apply subst_ext. intros []; unfold funcomp; now rewrite <- !sshift_spec.
   Qed.
 
   Lemma sat_sshift1 (rho : nat -> V) x y (phi : form) :
@@ -393,16 +406,13 @@ End Model.
 Lemma up_sshift1 (phi : form') sigma :
   phi[sshift 1][up (up sigma)] = phi[up sigma][sshift 1].
 Proof.
-  rewrite !subst_comp. apply subst_ext. intros []; trivial.
-  cbn. unfold funcomp. now destruct (sigma n) as [|[]].
+  unfold sshift. cbn. now asimpl.
 Qed.
 
 Lemma up_sshift2 (phi : form') sigma :
   phi[sshift 2][up (up (up sigma))] = phi[up sigma][sshift 2].
 Proof.
-  rewrite !subst_comp. apply subst_ext. intros [|[]]; trivial.
-  cbn. unfold funcomp. now destruct (sigma 0) as [|[]].
-  cbn. unfold funcomp. now destruct sigma as [|[]].
+  unfold sshift. cbn. now asimpl.
 Qed.
 
 Lemma rm_const_tm_subst (sigma : nat -> term') (t : term) :
@@ -437,13 +447,13 @@ Qed.
 Lemma eq_sshift1 (phi : form') t :
   phi[sshift 1][up t..] = phi.
 Proof.
-  erewrite subst_comp, subst_id; try reflexivity. now intros [].
+  unfold sshift. now asimpl.
 Qed.
 
 Lemma eq_sshift2 (phi : form') t :
   phi[sshift 2][up (up t..)] = phi[sshift 1].
 Proof.
-  erewrite subst_comp, subst_ext; try reflexivity. now intros [|].
+  unfold sshift. now asimpl.
 Qed.
 
 
@@ -1003,22 +1013,16 @@ Section Deduction.
     induction s in A, a, x |- *; cbn; try destruct F; cbn; intros HA Hx; try tauto.
     - destruct x0; cbn; try tauto. now apply rm_const_tm_equiv.
     - rewrite (vec_inv2 v). cbn. apply ex_equiv. intros B y HB. cbn. apply and_equiv.
-      + erewrite !subst_comp, subst_ext. setoid_rewrite subst_ext at 2.
-        apply IH; try apply in_hd. now rewrite HA. now apply (Weak Hx).
-        all: intros [|[]]; cbn; try reflexivity. apply subst_term_shift.
+      + unfold sshift. asimpl. apply IH; try apply in_hd. 1: intros k Hk; now apply HB,HA. now apply (Weak Hx).
       + apply ex_equiv. intros C z HC. cbn. apply and_equiv; try tauto.
-        erewrite !subst_comp, subst_ext. setoid_rewrite subst_ext at 2.
-        apply IH; try apply in_hd_tl. now rewrite HA, HB. apply (Weak Hx). now rewrite HB.
-        all: intros [|[]]; cbn; try reflexivity.
-        rewrite !subst_term_comp. now apply subst_term_id.
+        unfold sshift. asimpl. apply IH; try apply in_hd_tl.
+        now rewrite HA, HB. apply (Weak Hx). now rewrite HB.
     - rewrite (vec_inv1 v). cbn. apply ex_equiv. intros B y HB. cbn. apply and_equiv; try tauto.
-      erewrite !subst_comp, subst_ext. setoid_rewrite subst_ext at 2.
+      unfold sshift. asimpl. 
       apply IH; try apply in_hd. now rewrite HA. now apply (Weak Hx).
-      all: intros [|[]]; cbn; try reflexivity. apply subst_term_shift.
     - rewrite (vec_inv1 v). cbn. apply ex_equiv. intros B y HB. cbn. apply and_equiv; try tauto.
-      erewrite !subst_comp, subst_ext. setoid_rewrite subst_ext at 2.
+      unfold sshift. asimpl.
       apply IH; try apply in_hd. now rewrite HA. now apply (Weak Hx).
-      all: intros [|[]]; cbn; try reflexivity. apply subst_term_shift.
   Qed.
 
   Lemma rm_const_fm_swap { p : peirce } A phi t x :
@@ -1027,23 +1031,13 @@ Section Deduction.
     revert A. induction phi using form_ind_subst; cbn; intros A HA Hx.
     all: try destruct P0; try destruct b0; try destruct q; try tauto.
     - rewrite (vec_inv2 t0). cbn. apply ex_equiv. cbn. intros B a HB. apply and_equiv.
-      + rewrite subst_comp. erewrite subst_ext.
-        * eapply rm_const_tm_swap. now rewrite HA. now apply (Weak Hx).
-        * intros [|[|]]; trivial. now destruct x as [|[]].
+      + asimpl. eapply rm_const_tm_swap. now rewrite HA. now apply (Weak Hx).
       + apply ex_equiv. cbn. intros C a' HC. apply and_equiv; try tauto.
-        rewrite !subst_comp. erewrite subst_ext. setoid_rewrite subst_ext at 2.
-        * eapply rm_const_tm_swap. now rewrite HA, HB. apply (Weak Hx). now rewrite HB.
-        * intros [|[]]; reflexivity.
-        * intros [|[]]; trivial. now destruct x as [|[]].
+        unfold sshift. asimpl. eapply rm_const_tm_swap. now rewrite HA, HB. apply (Weak Hx). now rewrite HB.
     - rewrite (vec_inv2 t0). cbn. apply ex_equiv. cbn. intros B a HB. apply and_equiv.
-      + rewrite subst_comp. erewrite subst_ext.
-        * eapply rm_const_tm_swap. now rewrite HA. now apply (Weak Hx).
-        * intros [|[|]]; trivial. now destruct x as [|[]].
+      + asimpl. eapply rm_const_tm_swap. now rewrite HA. now apply (Weak Hx).
       + apply ex_equiv. cbn. intros C a' HC. apply and_equiv; try tauto.
-        rewrite !subst_comp. erewrite subst_ext. setoid_rewrite subst_ext at 2.
-        * eapply rm_const_tm_swap. now rewrite HA, HB. apply (Weak Hx). now rewrite HB.
-        * intros [|[]]; reflexivity.
-        * intros [|[]]; trivial. now destruct x as [|[]].
+        unfold sshift. asimpl. eapply rm_const_tm_swap. now rewrite HA, HB. apply (Weak Hx). now rewrite HB.
     - apply and_equiv; firstorder easy.
     - apply or_equiv; intros B HB.
       + apply IHphi1. now rewrite HA. now apply (Weak Hx).
@@ -1053,15 +1047,11 @@ Section Deduction.
       + apply IHphi2. now rewrite HA. now apply (Weak Hx).
     - apply all_equiv. intros [n|[]]. destruct x as [m|[]].
       assert (A ⊢ (rm_const_fm phi[$(S n)..])[$m..] <-> A ⊢ (rm_const_fm phi[$(S n)..][t..])) by now apply H, (Weak Hx).
-      erewrite subst_comp, subst_ext, <- subst_comp, (rm_const_fm_subst ($(S n)..)). setoid_rewrite subst_ext at 2.
-      rewrite H0. erewrite rm_const_fm_subst, !subst_comp, subst_ext. reflexivity.
-      all: intros [|[]]; cbn; try reflexivity. rewrite subst_term_comp, subst_term_id; reflexivity.
+      erewrite !rm_const_fm_subst. asimpl. asimpl in H0. erewrite rm_const_fm_subst in H0. asimpl in H0. apply H0.
     - apply ex_equiv. intros B s HB. destruct s as [n|[]], x as [m|[]].
       assert (B ⊢ (rm_const_fm phi[$(S n)..])[$m..] <-> B ⊢ (rm_const_fm phi[$(S n)..][t..])).
       { eapply H, (Weak Hx); trivial. now rewrite HA. }
-      erewrite subst_comp, subst_ext, <- subst_comp, (rm_const_fm_subst ($(S n)..)). setoid_rewrite subst_ext at 2.
-      rewrite H0. erewrite rm_const_fm_subst, !subst_comp, subst_ext. reflexivity.
-      all: intros [|[]]; cbn; try reflexivity. rewrite subst_term_comp, subst_term_id; reflexivity.
+      erewrite !rm_const_fm_subst. asimpl. asimpl in H0. erewrite rm_const_fm_subst in H0. asimpl in H0. apply H0.
   Qed.
 
   Lemma ZF_subst sigma :
