theories/FOL/FragmentSyntax.v
@@ -1,5 +1,5 @@
 From Undecidability.FOL Require Export
-  Syntax.Core Syntax.Facts
+  Syntax.Core Syntax.Facts Syntax.Asimpl
   Semantics.Tarski.FragmentFacts Semantics.Tarski.FragmentSoundness
   Semantics.Kripke.FragmentCore Semantics.Kripke.FragmentSoundness
   Semantics.Kripke.FragmentToTarski
