theories/FOL/FullSyntax.v
@@ -1,5 +1,5 @@
 From Undecidability.FOL Require Export
-  Syntax.Core Syntax.Facts
+  Syntax.Core Syntax.Facts Syntax.Asimpl
   Semantics.Tarski.FullFacts Semantics.Tarski.FullSoundness
   Deduction.FullNDFacts
   Semantics.FiniteTarski.Full.
